vale/code/arch/x64/interop/AES_stdcalls.fsti
@@ -21,6 +21,12 @@ let length_aux (b:uint8_p) : Lemma
     let db = get_downview b in
     DV.length_eq db
 
+let length_aux2 (b:uint8_p) : Lemma
+  (requires B.length b = 240)
+  (ensures DV.length (get_downview b) % 16 = 0) = 
+    let db = get_downview b in
+    DV.length_eq db
+
 inline_for_extraction
 val aes128_key_expansion
   (input_key_b:uint8_p)
@@ -43,3 +49,26 @@ val aes128_key_expansion
       length_aux output_key_expansion_b;
       let ub = UV.mk_buffer db Views.up_view128 in
       Seq.equal (UV.as_seq h1 ub) (key_to_round_keys_LE AES_128 key)))
+
+inline_for_extraction
+val aes256_key_expansion
+  (input_key_b:uint8_p)
+  (output_key_expansion_b:uint8_p)
+  : Stack unit
+    (requires fun h0 ->
+      B.disjoint input_key_b output_key_expansion_b /\
+
+      B.live h0 input_key_b /\ B.live h0 output_key_expansion_b /\
+
+      B.length input_key_b = 32 /\
+      B.length output_key_expansion_b = 240 /\
+
+      aesni_enabled)
+    (ensures fun h0 _ h1 ->
+      B.modifies (B.loc_buffer output_key_expansion_b) h0 h1 /\
+
+      (let key = seq_nat8_to_seq_nat32_LE (seq_uint8_to_seq_nat8 (B.as_seq h0 input_key_b)) in
+      let db = get_downview output_key_expansion_b in
+      length_aux2 output_key_expansion_b;
+      let ub = UV.mk_buffer db Views.up_view128 in
+      Seq.equal (UV.as_seq h1 ub) (key_to_round_keys_LE AES_256 key)))
