vale/code/arch/x64/interop/Gcm_simplify.fsti
@@ -12,6 +12,7 @@ open Words_s
 open Words.Seq_s
 open Vale.AsLowStar.MemoryHelpers
 open GCM_helpers
+open AES256_helpers
 open FStar.Mul
 
 val gcm_simplify1 (b:buf_t TUInt8 TUInt128) (h:HS.mem) (n:nat) : Lemma 
@@ -50,4 +51,13 @@ val aes_simplify1 (b:buf_t TUInt8 TUInt128) (h:HS.mem) : Lemma
   Seq.equal
     (seq_nat8_to_seq_nat32_LE (seq_uint8_to_seq_nat8 (B.as_seq h b)))
     (quad32_to_seq (low_buffer_read TUInt8 TUInt128 h b 0))
+  ))
+
+val aes_simplify2 (b:buf_t TUInt8 TUInt128) (h:HS.mem) : Lemma 
+  (requires B.live h b /\ B.length b = 32)
+  (ensures (
+  DV.length_eq (get_downview b);
+  Seq.equal
+    (seq_nat8_to_seq_nat32_LE (seq_uint8_to_seq_nat8 (B.as_seq h b)))
+    (make_AES256_key (low_buffer_read TUInt8 TUInt128 h b 0) (low_buffer_read TUInt8 TUInt128 h b 1))
   ))
